refine imp

src/Choice.v.d
@@ -1,0 +1,2 @@
+src/Choice.vo src/Choice.glob src/Choice.v.beautified: src/Choice.v src/Member.vo src/Comp.vo src/Eff.vo src/RWS.vo
+src/Choice.vio: src/Choice.v src/Member.vio src/Comp.vio src/Eff.vio src/RWS.vio
