src/Comp.v.d
@@ -1,0 +1,2 @@
+src/Comp.vo src/Comp.glob src/Comp.v.beautified: src/Comp.v
+src/Comp.vio: src/Comp.v
