src/Eff.v.d
@@ -1,0 +1,2 @@
+src/Eff.vo src/Eff.glob src/Eff.v.beautified: src/Eff.v src/Member.vo
+src/Eff.vio: src/Eff.v src/Member.vio
