src/Freer.v.d
@@ -1,0 +1,2 @@
+src/Freer.vo src/Freer.glob src/Freer.v.beautified: src/Freer.v
+src/Freer.vio: src/Freer.v
