src/Member.v.d
@@ -1,0 +1,2 @@
+src/Member.vo src/Member.glob src/Member.v.beautified: src/Member.v src/Freer.vo src/Union.vo
+src/Member.vio: src/Member.v src/Freer.vio src/Union.vio
