src/RWS.v.d
@@ -1,0 +1,2 @@
+src/RWS.vo src/RWS.glob src/RWS.v.beautified: src/RWS.v src/Eff.vo
+src/RWS.vio: src/RWS.v src/Eff.vio
