src/Refinement.v.d
@@ -1,0 +1,2 @@
+src/Refinement.vo src/Refinement.glob src/Refinement.v.beautified: src/Refinement.v
+src/Refinement.vio: src/Refinement.v
