src/Refine2.v
@@ -25,70 +25,79 @@ Definition nonDet_list : Eff [Choice] (list nat) :=
 Definition det_list: Eff [Choice] _ :=
      (pure (repeat 10 11)).
 
-Program Fixpoint denotes_choice {v} (s1: Eff [Choice] v) (s2: Eff [] v): Prop :=
+Fixpoint denotes_choice' {v} {effs} (s1: Eff (Choice :: effs) v) (s2: Eff [] v): Prop :=
   match s2 with
-  | Impure u _ => False_rect _ (Union_empty _ u)
+  | Impure u k => False_rect _ (Union_empty _ u)
   | Pure a2 =>
     match s1 with
     | Pure a1 => a1 = a2
     | Impure u1 k =>
-      match extract u1 with
-      | Pick p => exists a, denotes_choice (k a) s2 /\ p a
+      match decomp u1 with
+      | inl (Pick p) => exists a, denotes_choice' (k a) s2 /\ p a
+      | inr u' => exists a, denotes_choice' (k a) s2
       end
     end
   end.
 
+Fixpoint denotes_choice {v} {effs} (s1: Eff (Choice :: effs) v) (s2: Eff effs v): Prop :=
+  match s2 with
+  | Impure u k => exists a, denotes_choice s1 (k a) /\ ~ In Choice effs
+  | Pure a2 => denotes_choice' s1 (Pure a2)
+  end.
 
-Program Fixpoint denotes {v} (s1: Eff [Comp] v): Eff [] v -> Prop :=
+Fixpoint denotes_comp' {v} {effs} (s1: Eff (Comp :: effs) v): Eff [] v -> Prop :=
   fun s2 => match s2 with
   | Impure u _ => False_rect _ (Union_empty _ u)
   | Pure a2 =>
     match s1 with
     | Pure a1 => a1 = a2
     | Impure u1 k =>
-      match extract u1 with
-      | p => exists a, denotes (k a) s2 /\ p a
+      match decomp u1 with
+      | inl p => exists a, denotes_comp' (k a) s2 /\ p a
+      | inr u' => exists a, denotes_comp' (k a) s2
       end
     end
+  end.
+
+Fixpoint denotes_comp {v} {effs} (s1: Eff (Comp :: effs) v) (s2: Eff effs v): Prop :=
+  match s2 with
+  | Impure u k => exists a, denotes_comp s1 (k a) /\ ~ In Comp effs
+  | Pure a2 => denotes_comp' s1 (Pure a2)
   end.
 
 Lemma reduce_nonDet: 
   denotes_choice nonDet_list (pure (repeat 10 11)).
 Proof.
   intros.
-  remember (repeat 10 11) as l.
   simpl.
-  exists l.
-  subst; split; simpl; auto.
+  eexists.
+  split; eauto; simpl; eauto.
 Qed.
 
-Lemma nonEffect_Denotes: forall v (l: v),
-    denotes_choice (pure l) (pure l).
+Lemma nonEffect_Denotes: forall v effs (l: v),
+    @denotes_choice _ effs (pure l) (pure l).
 Proof.
   reflexivity.
 Qed.
 
-Lemma nonEffect_pure: forall v (l: v) x,
-    denotes_choice (pure l) x -> x = (pure l).
+Lemma nonEffect_pure: forall v x (l: v),
+    @denotes_choice _ nil (pure l) x -> x = (pure l).
 Proof.
-  intros.
-  simpl in *.
-  destruct x eqn:Heq in *; subst; auto.
-  inversion u.
+  destruct x; intros; simpl in *.
+  - subst.
+    reflexivity.
+  - inversion u.    
 Qed.
 
 Lemma pure_nonEffect: forall v (l: v) x,
-    x = (pure l) -> denotes_choice (pure l) x.
+    x = (pure l) -> @denotes_choice _ nil (pure l) x.
 Proof.
-  intros.
-  simpl in *.
-  destruct x eqn:Heq in *; subst; auto.
-  inversion H; auto.
-  inversion u.
+  intros; subst.
+  reflexivity.
 Qed.
 
 (* e1 refines e2 if forall t \in [| e2 |] -> t \in [| e1 |] *)
-Definition refines {v} e1 e2 := forall t, @denotes_choice v e2 t -> @denotes_choice v e1 t.
+Definition refines {v} {effs} e1 e2 := forall t, @denotes_choice v effs e2 t -> @denotes_choice v effs e1 t.
 
 Lemma refines_detList_nonDetList:
     refines nonDet_list det_list.
@@ -99,39 +108,147 @@ Proof.
   apply reduce_nonDet.
 Qed.
 
-Fixpoint pack_aexp (st: state) (a:aexp): Eff [Comp] nat :=
+Fixpoint denote_aexp {effs} (a:aexp): Eff ([State state]++effs) nat :=
   match a with
   | ANum n => pure n
-  | AId x => Impure (@UThis _ Comp _ (fun n => st x = n))
-                   (fun n => pure n)
+  | AId x => (st <- send Get;
+              pure (st x))
   | APlus a1 a2 | AMinus a1 a2 | AMult a1 a2
-                                 => pack_aexp st a1 ;; pack_aexp st a2
+                                 => denote_aexp a1 ;; denote_aexp a2
   end.
 
-Fixpoint pack_bexp (st: state) (b:bexp): Eff [Comp] bool :=
+Fixpoint denote_bexp {effs} (b:bexp): Eff ([State state]++effs) bool :=
   match b with
   | BTrue => pure true
   | BFalse => pure false
-  | BEq a1 a2 | BLe a1 a2 => (x1 <- (pack_aexp st a1) ;
-                               x2 <- (pack_aexp st a2) ;
+  | BEq a1 a2 | BLe a1 a2 => (x1 <- (denote_aexp a1) ;
+                               x2 <- (denote_aexp a2) ;
                                pure (beq_nat x1 x2))
-  | BAnd b1 b2 => (x1 <- pack_bexp st b1;
-                    x2 <- pack_bexp st b2;
+  | BAnd b1 b2 => (x1 <- (denote_bexp b1);
+                    x2 <- (denote_bexp b2);
                     pure (andb x1 x2))
-  | BNot b' => (b'' <- pack_bexp st b';
+  | BNot b' => (b'' <- denote_bexp b';
                  pure (negb b''))
   end.
 
-Fixpoint pack_imp (st: state) (c: com): Eff [Comp] state :=
+Fixpoint denote_imp {effs} (c: com): Eff ([State state]++effs) state :=
   match c with
-  | SKIP => pure st
-  | CAss x ax => (a <- pack_aexp st ax;
+  | SKIP => (st <- send Get; pure st)
+  | CAss x ax => (a <- denote_aexp ax;
+                   st <- send Get;
                    pure (t_update st x a))
-  | IFB b THEN c1 ELSE c2 FI => (b' <- pack_bexp st b;
-                                  c1' <- pack_imp st c1;
-                                  c2' <- pack_imp st c2;
-                                  pure (if b' then c1' else c2'))
-  | c1 ;;; c2 => pack_imp st c1 ;; pack_imp st c2
-  | WHILE b DO c' END => pure st
+  | IFB b THEN c1 ELSE c2 FI => b' <- denote_bexp b;
+                                 if (b':bool)
+                                 then denote_imp c1
+                                 else  denote_imp c2
+  | c1 ;;; c2 => denote_imp c1 ;; denote_imp c2
+  | WHILE b DO c' END => st <- send Get; pure st
   end.
 
+Inductive NDaexp: Type :=
+| Daexp : aexp -> NDaexp
+| NDnum : (Choice nat) -> NDaexp.
+
+Inductive NDbexp : Type :=
+| NBTrue : NDbexp
+| NBFalse : NDbexp
+| NBEq : NDaexp -> NDaexp -> NDbexp
+| NBLe : NDaexp -> NDaexp -> NDbexp
+| NBNot : NDbexp -> NDbexp
+| NBAnd : NDbexp -> NDbexp -> NDbexp.
+
+Inductive NDcom : Type :=
+| NDCSkip : NDcom
+| NDCAss : string -> NDaexp -> NDcom
+| NDCSeq : NDcom -> NDcom -> NDcom
+| NDCIf : NDbexp -> NDcom -> NDcom -> NDcom
+| NDCWhile : NDbexp -> NDcom -> NDcom.
+
+
+Fixpoint denote_NDaexp (na: NDaexp): Eff [State state; Choice] nat :=
+  match na with
+  | Daexp a => denote_aexp a
+  | NDnum (Pick p) => n <- send (Pick (fun (x: nat) => p x));
+              pure n
+  end.
+
+Fixpoint denote_NDbexp (nb:NDbexp): Eff [State state; Choice] bool :=
+  match nb with
+  | NBTrue => pure true
+  | NBFalse => pure false
+  | NBEq a1 a2 | NBLe a1 a2 => (x1 <- (denote_NDaexp a1) ;
+                               x2 <- (denote_NDaexp a2) ;
+                               pure (beq_nat x1 x2))
+  | NBAnd b1 b2 => (x1 <- (denote_NDbexp b1);
+                    x2 <- (denote_NDbexp b2);
+                    pure (andb x1 x2))
+  | NBNot b' => (b'' <- denote_NDbexp b';
+                 pure (negb b''))
+  end.
+
+Fixpoint denote_NDimp (nc: NDcom): Eff [State state; Choice] state :=
+  match nc with
+  | NDCSkip => (st <- send Get; pure st)
+  | NDCAss x ax => (a <- denote_NDaexp ax;
+                   st <- send Get;
+                   pure (t_update st x a))
+  | NDCIf b c1 c2 => b' <- denote_NDbexp b;
+                                 if (b':bool)
+                                 then denote_NDimp c1
+                                 else  denote_NDimp c2
+  | NDCSeq c1 c2 => denote_NDimp c1 ;; denote_NDimp c2
+  | NDCWhile b c' => st <- send Get; pure st
+  end.
+
+Definition effect_swap `(e: Eff ([eff1; eff2]++effs) v) : Eff ([eff2; eff1]++effs) v.
+Proof.
+  unfold Eff in *.
+  induction e.
+  - constructor; auto.
+  - inversion f; subst.
+    -- constructor 2 with x; auto.
+       constructor 2; eauto.
+       constructor 1; eauto.
+    -- inversion X0; subst.
+       --- constructor 2 with x; auto.
+           constructor; auto.
+       --- constructor 2 with x; auto.
+           repeat constructor 2.
+           auto.
+Defined.
+
+Notation "⇄ x" := (effect_swap x) (at level 50).
+Notation "⟦ c ⟧" := (denote_NDimp c) (at level 40).
+
+Definition plusNDet :=
+  ⇄ ⟦ NDCAss "X" (NDnum (Pick (fun x => x <= 2))) ⟧.
+
+Definition plusDet :=
+  ⇄ ⟦ NDCAss "X" (Daexp (ANum 2)) ⟧.
+
+Lemma refines_plusNDet_plusDet:
+  refines plusNDet plusDet.
+Proof.
+  unfold refines.
+  intros.
+  cbn in *.
+  induction t; simpl.
+  -- exists 2; eauto.
+  -- simpl in *.
+     destruct H.
+     exists x0.
+     destruct H.
+     split; auto.
+Qed.
+
+(* 1 V Denotes polimorphic on the rest of the effects
+   2 V Choice to aexp
+   3 V State in denote
+   4 V Write an Imp program with choice and show that you can refine to another without
+   5 - Formulate Heap operations in the Algebraic Effects
+   6 - Semantics of while with the Comp monad
+       -- look at the delay effect 
+       -- use fuel
+       -- encode the idea of fuel as an effect
+          -> show that any action in the presence of fuel terminates
+*)
