src/Eff.v
@@ -37,8 +37,6 @@ Definition send `{Member eff effs} `(t : eff a) : Eff effs a :=
   Impure (inj t) Pure.
 
 
-Obligation Tactic :=program_simpl.
-
 Program Fixpoint Eff_size `(q : Eff effs a)
         (P : forall eff r, FindElem eff effs -> eff r -> r) : nat :=
   match q with
